Add theorems for `std::default::Default` (#223)

stdlib/lampe/Stdlib/Default.lean
@@ -1,6 +1,269 @@
 import «std-1.0.0-beta.12».Extracted
+
 import Lampe
+import Stdlib.Tuple
 
 namespace Lampe.Stdlib.Default
 
 open «std-1.0.0-beta.12»
+open Lampe.Stdlib
+
+set_option Lampe.pp.Expr true
+set_option Lampe.pp.STHoare true
+
+/-- A shorthand for a call to the `std::default::Default::default` method. -/
+@[reducible]
+def default {p}
+    (generics : HList Kind.denote «std-1.0.0-beta.12::default::Default».«#genericKinds»)
+    (Self : Tp)
+    (associatedTypes : HList Kind.denote «std-1.0.0-beta.12::default::Default».«#associatedTypesKinds»)
+    (fnGenerics : HList Kind.denote «std-1.0.0-beta.12::default::Default».default.«#genericKinds»)
+  : HList (Tp.denote p)
+      («std-1.0.0-beta.12::default::Default».default.«#inputs» generics Self associatedTypes fnGenerics)
+  → Expr (Tp.denote p)
+      («std-1.0.0-beta.12::default::Default».default.«#output» generics Self associatedTypes fnGenerics) :=
+  «std-1.0.0-beta.12::default::Default».default generics Self associatedTypes fnGenerics
+
+/--
+Asserts that the provided `tp` has an implementation of `std::default::Default` in the environment.
+-/
+@[reducible]
+def hasDefaultImpl (env : Env) (tp : Tp) := «std-1.0.0-beta.12::default::Default».hasImpl env h![] tp
+
+theorem field_default_spec {p}
+  : STHoare p env ⟦⟧
+    (default h![] .field h![] h![] h![])
+    (fun r => r = 0) := by
+  resolve_trait
+  steps
+  simp_all
+
+theorem u1_default_spec {p}
+  : STHoare p env ⟦⟧
+    (default h![] (.u 1) h![] h![] h![])
+    (fun r => r = 0) := by
+  resolve_trait
+  steps
+  subst_vars
+  rfl
+
+theorem u8_default_spec {p}
+  : STHoare p env ⟦⟧
+    (default h![] (.u 8) h![] h![] h![])
+    (fun r => r = 0) := by
+  resolve_trait
+  steps
+  subst_vars
+  rfl
+
+theorem u16_default_spec {p}
+  : STHoare p env ⟦⟧
+    (default h![] (.u 16) h![] h![] h![])
+    (fun r => r = 0) := by
+  resolve_trait
+  steps
+  subst_vars
+  rfl
+
+theorem u32_default_spec {p}
+  : STHoare p env ⟦⟧
+    (default h![] (.u 32) h![] h![] h![])
+    (fun r => r = 0) := by
+  resolve_trait
+  steps
+  subst_vars
+  rfl
+
+theorem u64_default_spec {p}
+  : STHoare p env ⟦⟧
+    (default h![] (.u 64) h![] h![] h![])
+    (fun r => r = 0) := by
+  resolve_trait
+  steps
+  subst_vars
+  rfl
+
+theorem u128_default_spec {p}
+  : STHoare p env ⟦⟧
+    (default h![] (.u 128) h![] h![] h![])
+    (fun r => r = 0) := by
+  resolve_trait
+  steps
+  subst_vars
+  rfl
+
+theorem i8_default_spec {p}
+  : STHoare p env ⟦⟧
+    (default h![] (.i 8) h![] h![] h![])
+    (fun r => r = 0) := by
+  resolve_trait
+  steps
+  subst_vars
+  rfl
+
+theorem i16_default_spec {p}
+  : STHoare p env ⟦⟧
+    (default h![] (.i 16) h![] h![] h![])
+    (fun r => r = 0) := by
+  resolve_trait
+  steps
+  subst_vars
+  rfl
+
+theorem i32_default_spec {p}
+  : STHoare p env ⟦⟧
+    (default h![] (.i 32) h![] h![] h![])
+    (fun r => r = 0) := by
+  resolve_trait
+  steps
+  subst_vars
+  rfl
+
+theorem i64_default_spec {p}
+  : STHoare p env ⟦⟧
+    (default h![] (.i 64) h![] h![] h![])
+    (fun r => r = 0) := by
+  resolve_trait
+  steps
+  subst_vars
+  rfl
+
+theorem unit_default_spec {p}
+  : STHoare p env ⟦⟧
+    (default h![] .unit h![] h![] h![])
+    (fun r => r = 0) := by
+  resolve_trait
+  steps
+
+theorem bool_default_spec {p}
+  : STHoare p env ⟦⟧
+    (default h![] .bool h![] h![] h![])
+    (fun r => r = false) := by
+  resolve_trait
+  steps
+  simp_all
+
+theorem array_default_spec {p T N}
+    {t_default : hasDefaultImpl env T}
+    (t_default_emb : T.denote p)
+    (t_default_f : STHoare p env ⟦⟧
+      (default h![] T h![] h![] h![])
+      (fun r => r = t_default_emb))
+  : STHoare p env ⟦⟧
+    (default h![] (T.array N) h![] h![] h![])
+    (fun r => r = List.Vector.replicate N.toNat t_default_emb) := by
+  resolve_trait
+  steps [t_default_f]
+  simp_all
+
+theorem slice_default_spec {p}
+    {T : Tp}
+  : STHoare p env ⟦⟧
+    (default h![] T.slice h![] h![] h![])
+    (fun r => r = []) := by
+  resolve_trait
+  steps
+  simp_all
+
+theorem tuple2_default_spec {p A B}
+    {a_default : hasDefaultImpl env A}
+    (a_emb : A.denote p)
+    (a_sem : STHoare p env ⟦⟧
+      (default h![] A h![] h![] h![])
+      (fun r => r = a_emb))
+    {b_default : hasDefaultImpl env B}
+    (b_emb : B.denote p)
+    (b_sem : STHoare p env ⟦⟧
+      (default h![] B h![] h![] h![])
+      (fun r => r = b_emb))
+  : STHoare p env ⟦⟧
+    (default h![] (Tp.tuple none [A, B]) h![] h![] h![])
+    (fun r => r = Tuple.mk h![a_emb, b_emb]) := by
+  resolve_trait
+  steps [a_sem, b_sem]
+  simp_all
+
+theorem tuple3_default_spec {p A B C}
+    {a_default : hasDefaultImpl env A}
+    (a_emb : A.denote p)
+    (a_sem : STHoare p env ⟦⟧
+      (default h![] A h![] h![] h![])
+      (fun r => r = a_emb))
+    {b_default : hasDefaultImpl env B}
+    (b_emb : B.denote p)
+    (b_sem : STHoare p env ⟦⟧
+      (default h![] B h![] h![] h![])
+      (fun r => r = b_emb))
+    {c_default : hasDefaultImpl env C}
+    (c_emb : C.denote p)
+    (c_sem : STHoare p env ⟦⟧
+      (default h![] C h![] h![] h![])
+      (fun r => r = c_emb))
+  : STHoare p env ⟦⟧
+    (default h![] (Tp.tuple none [A, B, C]) h![] h![] h![])
+    (fun r => r = Tuple.mk h![a_emb, b_emb, c_emb]) := by
+  resolve_trait
+  steps [a_sem, b_sem, c_sem]
+  simp_all
+
+theorem tuple4_default_spec {p A B C D}
+    {a_default : hasDefaultImpl env A}
+    (a_emb : A.denote p)
+    (a_sem : STHoare p env ⟦⟧
+      (default h![] A h![] h![] h![])
+      (fun r => r = a_emb))
+    {b_default : hasDefaultImpl env B}
+    (b_emb : B.denote p)
+    (b_sem : STHoare p env ⟦⟧
+      (default h![] B h![] h![] h![])
+      (fun r => r = b_emb))
+    {c_default : hasDefaultImpl env C}
+    (c_emb : C.denote p)
+    (c_sem : STHoare p env ⟦⟧
+      (default h![] C h![] h![] h![])
+      (fun r => r = c_emb))
+    {d_default : hasDefaultImpl env D}
+    (d_emb : D.denote p)
+    (d_sem : STHoare p env ⟦⟧
+      (default h![] D h![] h![] h![])
+      (fun r => r = d_emb))
+  : STHoare p env ⟦⟧
+    (default h![] (Tp.tuple none [A, B, C, D]) h![] h![] h![])
+    (fun r => r = Tuple.mk h![a_emb, b_emb, c_emb, d_emb]) := by
+  resolve_trait
+  steps [a_sem, b_sem, c_sem, d_sem]
+  simp_all
+
+theorem tuple5_default_spec {p A B C D E}
+    {a_default : hasDefaultImpl env A}
+    (a_emb : A.denote p)
+    (a_sem : STHoare p env ⟦⟧
+      (default h![] A h![] h![] h![])
+      (fun r => r = a_emb))
+    {b_default : hasDefaultImpl env B}
+    (b_emb : B.denote p)
+    (b_sem : STHoare p env ⟦⟧
+      (default h![] B h![] h![] h![])
+      (fun r => r = b_emb))
+    {c_default : hasDefaultImpl env C}
+    (c_emb : C.denote p)
+    (c_sem : STHoare p env ⟦⟧
+      (default h![] C h![] h![] h![])
+      (fun r => r = c_emb))
+    {d_default : hasDefaultImpl env D}
+    (d_emb : D.denote p)
+    (d_sem : STHoare p env ⟦⟧
+      (default h![] D h![] h![] h![])
+      (fun r => r = d_emb))
+    {e_default : hasDefaultImpl env E}
+    (e_emb : E.denote p)
+    (e_sem : STHoare p env ⟦⟧
+      (default h![] E h![] h![] h![])
+      (fun r => r = e_emb))
+  : STHoare p env ⟦⟧
+    (default h![] (Tp.tuple none [A, B, C, D, E]) h![] h![] h![])
+    (fun r => r = Tuple.mk h![a_emb, b_emb, c_emb, d_emb, e_emb]) := by
+  resolve_trait
+  steps [a_sem, b_sem, c_sem, d_sem, e_sem]
+  simp_all
+
